iris/ProofPipealloc.v
@@ -28,7 +28,7 @@ From Stdlib Require Import Eqdep_dec ZArith Lia List.
 From stdpp Require Import gmap list list_monad bitvector.definitions bitvector.tactics.
 From iris.proofmode Require Import proofmode.
 From iris.algebra Require Import excl auth gmap frac numbers.
-From iris.base_logic.lib Require Import ghost_var gen_heap invariants.
+From iris.base_logic.lib Require Import cancelable_invariants ghost_var gen_heap invariants.
 From iris.program_logic Require Import language weakestpre lifting.
 Require Import SailStdpp.ConcurrencyInterface SailStdpp.ConcurrencyInterfaceBuiltins SailStdpp.ConcurrencyInterfaceTypes SailStdpp.Operators_mwords.
 Require Import Riscv.rv64d_types Riscv.rv64d Riscv.riscv_extras.
@@ -86,7 +86,7 @@ Module PipeallocProof (Filealloc : FILEALLOC) (Kalloc : KALLOC)
                       (Initlock : INITLOCK) (Fileclose : FILECLOSE) : PIPEALLOC.
 
 Section ProofPipealloc.
-  Context `{!riscvGS Σ, !lockG Σ, !sieG Σ, !fileG Σ, !fdslotG Σ, !kallocG Σ, !pipeG Σ}.
+  Context `{!riscvGS Σ, !lockG Σ, !sieG Σ, !fileG Σ, !fdslotG Σ, !kallocG Σ, !pipeG Σ, !cinvG Σ}.
   Context `{CID : CpuId}.
 
   Notation PA := KernelSyms.pipealloc.
@@ -1347,13 +1347,13 @@ Section ProofPipealloc.
     assert (Hpc54 : ret_pc (G5 !!! Regidx Rra) = mword_of_int (PA + 0x54))
       by (rewrite HG5ra; apply bv_eq; vm_compute; reflexivity).
     iEval (rewrite Hpc54) in "Hpc".
-    iEval (rewrite HG5a0) in "Hlkw". iEval (rewrite HG5a0 HG5a1) in "Hlkn".
+    iEval (rewrite HG5a0) in "Hlkw". iEval (rewrite HG5a0) in "Hlkn".
     iEval (rewrite HG5a0) in "Hlkc".
-    iMod (lock_name_intro with "Hstr Hlkn") as "#Hlnm".
-    (* the pipe is born *)
+    (* the pipe is born.  The lock's name field goes INTO the pipe rather than
+       being sealed away: it is 8 bytes of the page pipeclose has to free. *)
     iApply fupd_wp.
-    iMod (new_pipe ⊤ pi bs Hpv Hbslen
-            with "Hlnm Hlkw Hlkc Hnr Hnw Hro Hwo Hdat Hslack") as (γpl γp) "(#Hpipe & Hrd & Hwr)".
+    iMod (new_pipe ⊤ pi _ bs Hpv Hbslen
+            with "Hlkn Hlkw Hlkc Hnr Hnw Hro Hwo Hdat Hslack") as (γpl γp) "(#Hpipe & Hrd & Hwr)".
     iModIntro.
 
     (* ---- the eight unlocked stores into the two struct files ---- *)
